src/mem/Program.v
@@ -1,0 +1,41 @@
+Require Import sflib.
+
+Require Import Basic.
+Require Import Thread.
+Require Import Memory.
+Require Import Configuration.
+
+Set Implicit Arguments.
+
+Module Program.
+  Structure thread_t := thread_mk {
+    lang: Language.t;
+    text: lang.(Language.text);
+  }.
+
+  Definition t := IdentMap.t thread_t.
+
+  Inductive load_thread: forall (text:thread_t) (th:Thread.t), Prop :=
+  | load_thread_intro
+      lang text s
+      (LOAD: lang.(Language.load) text s):
+      load_thread (thread_mk lang text) (Thread.mk lang s)
+  .
+
+  Inductive load_threads (text:t) (th:Threads.t): Prop :=
+  | load_threads_intro
+      (LOAD:
+         forall i,
+           <<NONE: IdentMap.find i text = None /\ IdentMap.find i th = None>> \/
+           <<SOME: exists text' th',
+                     <<TEXT: IdentMap.find i text = Some text'>> /\
+                     <<THREAD: IdentMap.find i th = Some th'>> /\
+                     <<LOAD: load_thread text' th'>>>>)
+  .
+
+  Inductive load: forall (text:t) (c:Configuration.t), Prop :=
+  | load_intro
+      text th (LOAD: load_threads text th):
+      load text (Configuration.mk Clocks.init th Memory.empty nil)
+  .
+End Program.
