src/sim/Simulation.v
@@ -1,0 +1,77 @@
+Require Import sflib.
+
+Require Import Event.
+Require Import Configuration.
+Require Import Program.
+
+Set Implicit Arguments.
+
+Inductive tausteps: forall (src:Configuration.t) (src':Configuration.t), Prop :=
+| tausteps_nil
+    src:
+    tausteps src src
+| tausteps_cons
+    src src' src''
+    (STEP: Configuration.step src None src')
+    (STEPS: tausteps src' src''):
+    tausteps src src''
+.
+
+Inductive srcsteps: forall (src:Configuration.t) (e:option Event.t) (src':Configuration.t), Prop :=
+| srcsteps_stationary
+    src src'
+    (TAU: tausteps src src'):
+    srcsteps src None src'
+| srcsteps_progress
+    src src' src'' e
+    (TAU: tausteps src src')
+    (PROGRESS: Configuration.step src' e src''):
+    srcsteps src e src''
+.
+
+(* TODO: proper use of indexes *)
+Module Simulation.
+  Section Simulation.
+    Variable (prog_src prog_tgt:Program.t).
+    Variable (sim: forall (src tgt:Configuration.t), Prop).
+
+    Definition LOAD: Prop :=
+      forall tgt (TGT: Program.load prog_tgt tgt),
+      exists src,
+        <<SRC: Program.load prog_src src>> /\
+        <<SIM: sim src tgt>>.
+
+    Definition STEP: Prop :=
+      forall src tgt e tgt'
+        (SIM: sim src tgt)
+        (STEP: Configuration.step tgt e tgt'),
+      exists src',
+        <<STEP: srcsteps src e src'>> /\
+                <<SIM: sim src' tgt'>>.
+
+    Definition OBSERVABLE: Prop :=
+      forall src tgt
+        (SIM: sim src tgt)
+        (TERM: Configuration.is_observable tgt),
+      exists src',
+        <<STEP: tausteps src src'>> /\
+        <<TERM: Configuration.is_observable src'>>.
+
+    Definition TERMINAL: Prop :=
+      forall src tgt
+        (SIM: sim src tgt)
+        (TERM: Configuration.is_terminal tgt),
+      exists src',
+        <<STEP: tausteps src src'>> /\
+        <<TERM: Configuration.is_terminal src'>>.
+  End Simulation.
+
+  Structure t (prog_src prog_tgt:Program.t) := mk {
+    sim: forall (src tgt:Configuration.t), Prop;
+
+    load: LOAD prog_src prog_tgt sim;
+    step: STEP sim;
+    observable: OBSERVABLE sim;
+    terminal: TERMINAL sim;
+  }.
+End Simulation.
